Arithmetization/ISigmaOne/PRF.lean
@@ -114,7 +114,7 @@ lemma CSeq.initial : c.CSeq v !⟨c.zero v⟩ :=
   ⟨by simp, by simp [seqCons], by simp⟩
 
 lemma CSeq.successor {s l z : M} (Hs : c.CSeq v s) (hl : l + 1 = lh s) (hz : ⟪l, z⟫ ∈ s) :
-    c.CSeq v (c.succ v l z ::ˢ s) :=
+    c.CSeq v (s ⁀' c.succ v l z) :=
   ⟨ Hs.seq.seqCons _, by simp [seqCons, Hs.zero], by
     simp [Hs.seq.lh_seqCons]
     intro i hi w hiw
@@ -145,7 +145,7 @@ lemma CSeq.exists (l : M) : ∃ s, c.CSeq v s ∧ l + 1 = lh s := by
     have hl : l < lh s := by simp [←hls]
     have : ∃ z, ⟪l, z⟫ ∈ s := Hs.seq.exists hl
     rcases this with ⟨z, hz⟩
-    exact ⟨c.succ v l z ::ˢ s, Hs.successor hls hz, by simp [Hs.seq, hls]⟩
+    exact ⟨s ⁀' c.succ v l z, Hs.successor hls hz, by simp [Hs.seq, hls]⟩
 
 lemma cSeq_result_existsUnique (l : M) : ∃! z, ∃ s, c.CSeq v s ∧ l + 1 = lh s ∧ ⟪l, z⟫ ∈ s := by
   rcases CSeq.exists c v l with ⟨s, Hs, h⟩
@@ -166,7 +166,7 @@ lemma result_spec (u : M) : ∃ s, c.CSeq v s ∧ u + 1 = lh s ∧ ⟪u, c.resul
 
 @[simp] theorem result_succ (u : M) : c.result v (u + 1) = c.succ v u (c.result v u) := by
   rcases c.result_spec v u with ⟨s, Hs, hk, h⟩
-  have : CSeq c v (c.succ v u (result c v u) ::ˢ s) := Hs.successor hk h
+  have : CSeq c v (s ⁀' c.succ v u (result c v u) ) := Hs.successor hk h
   exact Eq.symm
     <| Classical.choose_uniq (c.cSeq_result_existsUnique v (u + 1))
     ⟨_, this, by simp [Hs.seq, hk], by simp [hk]⟩
@@ -201,6 +201,111 @@ instance result_definable_delta₁ : DefinableFunction ℒₒᵣ 𝚫₁ (fun v 
 end Construction
 
 end PR
+
+section seqExp
+
+lemma seqCons_le {x y s t : M} (hxy : x ≤ y) (hst : s ≤ t) :
+    s ⁀' x ≤ t + exp ((2 * t + y + 1)^2) := by
+  have : s ⁀' x ≤ t + exp ⟪2 * t, y⟫ := by
+    simp [seqCons]; exact insert_le_of_le_of_le (pair_le_pair (le_trans (lh_bound s) (by simp [hst])) hxy) hst
+  exact le_trans this (by simp)
+
+lemma seqProduct_exists_unique (s a : M) : ∃! t : M, ∀ x, x ∈ t ↔ ∃ v ∈ s, ∃ u ∈ a, x = v ⁀' u := by
+  have : 𝚺₁-Predicate fun x ↦ ∃ v ∈ s, ∃ u ∈ a, x = v ⁀' u := by definability
+  exact finite_comprehension₁! this ⟨log s + exp ((2 * log s + log a + 1)^2) + 1, by
+    rintro x ⟨v, hv, u, hu, rfl⟩
+    exact lt_succ_iff_le.mpr <| seqCons_le (le_log_of_mem hu) (le_log_of_mem hv)⟩
+
+def seqProduct (a s : M) : M := Classical.choose! (seqProduct_exists_unique a s)
+
+infixl:60 " ×ˢ " => seqProduct
+
+lemma mem_seqProduct_iff {x s a : M} : x ∈ s ×ˢ a ↔ ∃ v ∈ s, ∃ u ∈ a, x = v ⁀' u :=
+  Classical.choose!_spec (seqProduct_exists_unique s a) x
+
+lemma mem_seqProduct_iff' {u v a s : M} (Hv : Seq v) (Hs : ∀ w ∈ s, Seq w) :
+    v ⁀' u ∈ s ×ˢ a ↔ v ∈ s ∧ u ∈ a :=
+  ⟨by intro h
+      rcases mem_seqProduct_iff.mp h with ⟨v', hv', u', hu', e⟩
+      have : u = u' ∧ v = v' := by simpa [Hv, Hs v' hv'] using e
+      rcases this with ⟨rfl, rfl⟩
+      constructor <;> assumption,
+   by rintro ⟨hv, hu⟩
+      exact mem_seqProduct_iff.mpr ⟨v, hv, u, hu, rfl⟩⟩
+
+lemma mem_seqProduct_bound {x s a : M} (h : x ∈ s ×ˢ a) : x ≤ s + exp ((2 * s + a + 1)^2) := by
+  rcases mem_seqProduct_iff.mp h with ⟨v, hv, u, hu, rfl⟩
+  exact seqCons_le (le_of_lt <| lt_of_mem hu) (le_of_lt <| lt_of_mem hv)
+
+private lemma seqProduct_graph (t s a : M) : t = s ×ˢ a ↔ ∃ e, e = exp ((2 * s + a + 1)^2) ∧ ∀ x < t + s + e + 1, x ∈ t ↔ ∃ v ∈ s, ∃ u ∈ a, x = v ⁀' u :=
+⟨by rintro rfl; exact ⟨exp ((2 * s + a + 1)^2), rfl, by intro x _; simp [mem_seqProduct_iff]⟩,
+ by rintro ⟨_, rfl, h⟩
+    apply mem_ext; intro x
+    constructor
+    · intro hx;
+      exact mem_seqProduct_iff.mpr
+        <| h x (lt_of_lt_of_le (lt_of_mem hx) (by simp [add_assoc])) |>.mp hx
+    · intro hx
+      exact h x (lt_succ_iff_le.mpr <| le_trans (mem_seqProduct_bound hx) <| by simp [add_assoc])
+        |>.mpr (mem_seqProduct_iff.mp hx)⟩
+
+def _root_.LO.FirstOrder.Arith.seqProductDef : 𝚺₁-Semisentence 3 := .mkSigma
+  “∃ (!expDef.val [#0, (2 * #2 + #3 + 1 ) ^' 2] ∧
+    ∀[#0 < #2 + #3 + #1 + 1] ( #0 ∈ #2 ↔ [∃∈ #3] [∃∈ #5] !seqConsDef.val [#2, #1, #0] ) )”
+  (by simp [Hierarchy.iff_iff])
+
+lemma seqProduct_defined : 𝚺₁-Function₂ (seqProduct : M → M → M) via seqProductDef := by
+  intro v; simp [seqProductDef, seqProduct_graph]
+
+@[simp] lemma seqProduct_defined_iff (v) :
+    Semiformula.Evalbm M v seqProductDef.val ↔ v 0 = v 1 ×ˢ v 2 := seqProduct_defined.df.iff v
+
+instance seqProduct_definable : 𝚺₁-Function₂ (seqProduct : M → M → M) := Defined.to_definable _ seqProduct_defined
+
+def seqExp.formulae : PR.Formulae 1 where
+  zero := .mkSigma “#0 = 1” (by simp)
+  succ := .mkSigma “!seqProductDef.val [#0, #1, #3]” (by simp)
+
+def seqExp.construction : PR.Construction M seqExp.formulae where
+  zero := fun _ ↦ {∅}
+  succ := fun a _ s ↦ s ×ˢ a 0
+  zero_defined := by intro v; simp [formulae, one_eq_singleton]
+  succ_defined := by intro v; simp [formulae]; rfl
+
+def seqExp (a k : M) : M := seqExp.construction.result ![a] k
+
+infix:80 " ^ˢ " => seqExp
+
+@[simp] lemma seqExp_zero (a : M) : a ^ˢ 0 = {∅} := by simp [seqExp, seqExp.construction]
+
+@[simp] lemma seqExp_succ (a k : M) : a ^ˢ (k + 1) = (a ^ˢ k) ×ˢ a := by simp [seqExp, seqExp.construction]
+
+def _root_.LO.FirstOrder.Arith.seqExpDef : 𝚫₁-Semisentence 3 := seqExp.formulae.resultDef |>.rew (Rew.substs ![#0, #2, #1]) |>.graphDelta
+
+lemma seqExp_defined : 𝚫₁-Function₂ (seqExp : M → M → M) via seqExpDef := by
+  apply DefinedFunction.graph_delta <| fun v ↦ by simp [seqExp.construction.result_defined_iff]; rfl
+
+@[simp] lemma seqExp_defined_iff (v) :
+    Semiformula.Evalbm M v seqExpDef.val ↔ v 0 = v 1 ^ˢ v 2 := seqExp_defined.df.iff v
+
+instance seqExp_definable : 𝚫₁-Function₂ (seqExp : M → M → M) := Defined.to_definable _ seqExp_defined
+
+@[simp, definability] instance seqExp_definable' (Γ) : (Γ, 1)-Function₂ (seqExp : M → M → M) := .of_delta seqExp_definable
+
+attribute [definability] DefinableFunction₂.comp
+
+lemma seq_of_mem_seqExp {s a k : M} (h : s ∈ seqExp a k) : Seq s := by
+  induction k using induction_iSigmaOne generalizing s
+  · sorry
+  case zero =>
+    have : s = ∅ := by simpa using h
+    simp [this]
+  case succ k ih =>
+    have : ∃ v ∈ a ^ˢ k, ∃ u ∈ a, s = v ⁀' u := by simpa [mem_seqProduct_iff] using h
+    rcases this with ⟨v, hv, u, hu, rfl⟩
+    exact (ih hv).seqCons u
+
+end seqExp
 
 end LO.FirstOrder.Arith.Model
 
